pulse/src/checker/Pulse.Checker.WithLocalArray.fst
@@ -90,7 +90,8 @@ let check
       "Allocating a mutable local variable expects an annotated post-condition"
 
   | Some { effect_annot = EffectAnnotGhost _ }
-  | Some { effect_annot = EffectAnnotAtomic _ } ->
+  | Some { effect_annot = EffectAnnotAtomic _ }
+  | Some { effect_annot = EffectAnnotAtomicOrGhost _ } ->
     fail g (Some <| head_range t)
       "Allocating a mutable local variable is only allowed in non-ghost and non-atomic code"
   
